engine/PrisonersDilemma.lean
@@ -1,6 +1,9 @@
 -- This module serves as the root of the `PrisonersDilemma` library.
 -- Import modules here that should be built as part of the library.
 import PrisonersDilemma.SizeLemmas
+import PrisonersDilemma.ComputableEval.Computable
+import PrisonersDilemma.ComputableEval.Demo
+import PrisonersDilemma.ComputableEval.DecMeasure
 import PrisonersDilemma.Theorems.CupodBot
 import PrisonersDilemma.Theorems.CooperateBot
 import PrisonersDilemma.Theorems.DefectBot
